# Saved by TopBraid on Fri Aug 06 16:36:04 CEST 2010
# baseURI: http://purl.org/ontology/ao/core#
# imports: http://purl.org/dc/elements/1.1/
# imports: http://purl.org/ontology/similarity/
# imports: http://www.w3.org/2003/06/sw-vocab-status/ns
# imports: http://purl.org/stuff/rev
# imports: http://www.w3.org/2004/03/trix/rdfg-1/
# imports: http://xmlns.com/foaf/0.1/
# imports: http://purl.org/dc/terms/

@prefix ao:      <http://purl.org/ontology/ao/core#> .
@prefix dc:      <http://purl.org/dc/elements/1.1/> .
@prefix dcterms:  <http://purl.org/dc/terms/> .
@prefix foaf:    <http://xmlns.com/foaf/0.1/> .
@prefix owl:     <http://www.w3.org/2002/07/owl#> .
@prefix rdf:     <http://www.w3.org/1999/02/22-rdf-syntax-ns#> .
@prefix rdfg:    <http://www.w3.org/2004/03/trix/rdfg-1/> .
@prefix rdfs:    <http://www.w3.org/2000/01/rdf-schema#> .
@prefix rev:     <http://purl.org/stuff/rev#> .
@prefix sim:     <http://purl.org/ontology/similarity/> .
@prefix vs:      <http://www.w3.org/2003/06/sw-vocab-status/ns#> .
@prefix xsd:     <http://www.w3.org/2001/XMLSchema#> .

ao:   rdf:type owl:Ontology ;
      dc:creator <http://foaf.me/zazi#me> ;
      dc:date "2010-08-06T15:35:52+01:00"^^xsd:dateTime ;
      dc:description """The Association Ontology specification provides basic properties 
for describing specific associations to something, e.g. an occasion, a genre or a mood, and enables furthermore, a mechanism to 
like/rate and feedback these associations in context to something on/ for the Semantic Web. This document contains a RDF description 
of the Association Ontology."""@en ;
      dc:title "The Association Ontology"@en ;
      owl:imports rdfg: , dcterms: , <http://purl.org/stuff/rev> , dc: , <http://www.w3.org/2003/06/sw-vocab-status/ns> , sim: , foaf: ;
      owl:versionInfo 0.3 .

ao:LikeableAssociation
      rdf:type owl:Class ;
      rdfs:comment """A likeable association. That means this association type is intended to be used for voting (ao:likeminded), 
feedbacking (rev:Feedback), reviewing (e.g. rev:rating) an association statement (related by ao:included_association) in the 
context of something."""@en ;
      rdfs:isDefinedBy ao: ;
      rdfs:label "Likeable Association"@en ;
      rdfs:subClassOf sim:Association , rev:Review ;
      vs:term_status "testing"@en .

ao:associates
      rdf:type rdf:Property , owl:ObjectProperty ;
      rdfs:comment "Related the graph of the association statement, which describes the subjective associations."@en ;
      rdfs:domain sim:Association ;
      rdfs:isDefinedBy ao: ;
      rdfs:label "associates"@en ;
      rdfs:range rdfg:Graph ;
      vs:term_status "testing"@en .

ao:genre
      rdf:type rdf:Property ;
      rdfs:comment "An genre of something."@en ;
      rdfs:domain owl:Thing ;
      rdfs:isDefinedBy ao: ;
      rdfs:label "has genre"@en ;
      rdfs:subPropertyOf dcterms:subject ;
      vs:term_status "unstable"@en .

ao:included_association
      rdf:type owl:ObjectProperty ;
      rdfs:comment """This property could be used to compose association statements or to reuse them, e.g. to make them likeable 
in a specific context."""@en ;
      rdfs:domain sim:Association ;
      rdfs:isDefinedBy ao: ;
      rdfs:label "has included association"@en ;
      rdfs:range sim:Association ;
      owl:inverseOf
              [ rdf:type owl:ObjectProperty ;
                rdfs:label "is included association of"
              ] ;
      vs:term_status "testing"@en .

ao:likeminded
      rdf:type owl:ObjectProperty ;
      rdfs:comment "Associates likeminded people to an association, which they like/ agree with."^^xsd:string ;
      rdfs:domain sim:Association ;
      rdfs:isDefinedBy ao: ;
      rdfs:label "has likeminded"^^xsd:string ;
      rdfs:range foaf:Agent ;
      owl:inverseOf
              [ rdf:type owl:ObjectProperty ;
                rdfs:label "is likeminded of"
              ] ;
      vs:term_status "testing"^^xsd:string .

ao:mood
      rdf:type rdf:Property ;
      rdfs:comment "A mood that should be created by something."@en ;
      rdfs:domain owl:Thing ;
      rdfs:isDefinedBy ao: ;
      rdfs:label "has mood"@en ;
      rdfs:subPropertyOf dcterms:subject ;
      vs:term_status "unstable"@en .

ao:occasion
      rdf:type rdf:Property ;
      rdfs:comment "An occasion for which something was created."@en ;
      rdfs:domain owl:Thing ;
      rdfs:isDefinedBy ao: ;
      rdfs:label "has occassion"@en ;
      rdfs:subPropertyOf dcterms:subject ;
      vs:term_status "unstable"@en .

ao:substitution
      rdf:type rdf:Property ;
      rdfs:comment "A class instances would be substituted by another class instances to enable statements, which are independent from a specific class instance."^^xsd:string ;
      rdfs:domain owl:Thing ;
      rdfs:isDefinedBy ao: ;
      rdfs:label "substitution"^^xsd:string ;
      rdfs:range owl:Thing ;
      vs:term_status "testing"^^xsd:string .
